$$
    f(x) = \sqrt{x - 2} - 1
$$

`Dominio`: $[2, \infty) \in \mathbb{R}$

`Rango`: $[-1, \infty) \in \mathbb{R}$


#### Encontrar la inversa

despejamos $x$ en funcion de $y$

$$
    f(x) = y = \sqrt{x - 2} - 1
$$
$$
    y + 1 = \sqrt{x - 2}
$$
$$
    (y + 1)^{2} = \left( \sqrt{x - 2} \right)^{2}
$$
$$
    (y + 1)^{2} = x - 2
$$
$$
    (y + 1)^{2} + 2 = x 
$$
$$
    x = (y + 1)^{2} + 2  
$$

Aplicamos el cambio de varible

$$
    f^{-1}(x) = (x + 1)^{2} + 2  
$$

`Dominio`: $[-1, \infty) \in \mathbb{R}$

`Rango`: $[2, \infty) \in \mathbb{R}$

