---
geogebra: [
    {id: 'hnd2ttnn', title: ''}
]
---

# Ejemplo 1

$$
    f(x) = \sqrt{1 - x}
$$

$$
    g(x) = \sqrt{x + 1}
$$

## Dominio

- ##### Dominio de $f$:
    $$
        1 - x \geq 0 \hspace{20pt} 1 \geq x
    $$
    $$
        \text{Dom } f = \left\{ x \leq 1  \right\} = (-\infty, 1]
    $$

<br />

- ##### Dominio de $g$:
    $$
        x + 1 \geq 0 \hspace{20pt} x \geq -1
    $$
    $$
        \text{Dom } g = \left\{ x \geq -1  \right\} = [-1, \infty)
    $$

- ##### Interseccion

    $$
        \text{Dom } f \cap \text{Dom } g = (-\infty, 1] \cap [-1, \infty) = [-1, 1]
    $$

<br />

## Algebra de funciones

$$
\text{Dom } f \cap \text{Dom } g = [-1, 1] \neq \varnothing
$$

Por lo tanto existe:


- $f + g$

    $$
        (f + g)(x) = \sqrt{1 - x} + \sqrt{x + 1}
    $$
    con `dominio` en: $[-1, 1]$

--------
<br />

- $f - g$

    $$
        (f - g)(x) = \sqrt{1 - x} - \sqrt{x + 1}
    $$
    con `dominio` en: $[-1, 1]$

--------
<br />

- $g - f$

    $$
        (g - f)(x) = \sqrt{x + 1} - \sqrt{1 - x}
    $$
    con `dominio` en: $[-1, 1]$

--------
<br />

- $f \cdot g$

    $$
        (f \cdot g)(x) = \sqrt{(1 - x) \cdot (x + 1)}
    $$
    con `dominio` en: $[-1, 1]$

--------
<br />

- $f / g$

    $$
        \left( \frac{f}{g} \right)(x) = \left( \frac{\sqrt{1 - x}}{\sqrt{x + 1}} \right)
    $$
    con `dominio` en: $(-1, 1]$

--------
<br />

- $g / f$

    $$
        \left( \frac{g}{f} \right)(x) = \left( \frac{\sqrt{x + 1}}{\sqrt{1 - x}} \right)
    $$
    con `dominio` en: $[-1, 1)$