

$$
    f(x) = 2 \cdot x - 4
$$

Encontrar la derivada aplicando la definicion

$$
    \begin{array}{c}
        \displaystyle{
            f'(x) = \lim_{h \to 0} \frac{f(x + h) - f(x)}{h}
        }
        \\\\
        \displaystyle{
           f'(x) = \lim_{h \to 0}
           \frac{
                (2 \cdot (x + h) - 4) - (2 \cdot x - 4)
            }{h} 
        }
        \\\\
        \displaystyle{
           f'(x) = \lim_{h \to 0}
           \frac{
                2 \cdot x + 2 \cdot h - 4 - 2 \cdot x + 4
            }{h} 
        }
        \\\\
        \displaystyle{
           f'(x) = \lim_{h \to 0}
           \frac{
                \cancel{2 \cdot x} + 2 \cdot h - \cancel{4} - \cancel{2 \cdot x} + \cancel{4}
            }{h} 
        }
        \\\\
        \displaystyle{
           f'(x) = \lim_{h \to 0}
           \frac{2 \cdot h}{h} 
        }
        \\\\
        \displaystyle{
           f'(x) = \lim_{h \to 0}
           \frac{2 \cdot \cancel{h}}{\cancel{h}} 
        }
        \\\\
        \displaystyle{
           f'(x) = \lim_{h \to 0} 2
        }
    \end{array}
$$

Resolvemos el limite

$$
    f'(x) = \lim_{h \to 0} 2 = 2 
$$

Finalmente la derivada es

$$
    f'(x) = 2 
$$

---
<br>

$$
    f(x) = x^{2}
$$

Encontrar la derivada aplicando la definicion

$$
    \begin{array}{c}
        \displaystyle{
            f'(x) = \lim_{h \to 0} \frac{f(x + h) - f(x)}{h}
        }
        \\\\
        \displaystyle{
           f'(x) = \lim_{h \to 0}
           \frac{
                (x + h)^{2} - x^{2}
            }{h} 
        }
        \\\\
        \displaystyle{
           f'(x) = \lim_{h \to 0}
           \frac{
                x^{2} + 2 \cdot x \cdot h + h^{2} - x^{2}
            }{h} 
        }
        \\\\
        \displaystyle{
           f'(x) = \lim_{h \to 0}
           \frac{
                \cancel{x^{2}} + 2 \cdot x \cdot h + h^{2} - \cancel{x^{2}}
            }{h} 
        }
        \\\\
        \displaystyle{
           f'(x) = \lim_{h \to 0}
           \frac{2 \cdot x \cdot h + h^{2}}{h} 
        }
        \\\\
        \displaystyle{
           f'(x) = \lim_{h \to 0}
           \frac{h \cdot (2 \cdot x + h)}{h} 
        }
        \\\\
        \displaystyle{
           f'(x) = \lim_{h \to 0}
           \frac{\cancel{h} \cdot (2 \cdot x + h)}{\cancel{h}}  
        }
        \\\\
        \displaystyle{
           f'(x) = \lim_{h \to 0} 2 \cdot x + h
        }
    \end{array}
$$

Resolvemos el limite

$$
    f'(x) = \lim_{h \to 0} 2 \cdot x + h = 2 \cdot x
$$

Finalmente la derivada es

$$
    f'(x) = 2 \cdot x
$$