## Teorema del resto - ejemplo 1

$$
    \frac{4 \cdot x^{40} + 8 \cdot x^{39} + 1}{x + 2}
$$

Igualar el denominador a $0$

$$
    x + 2 = 0
$$
$$
    x = -2
$$

Calcular el `resto` evaluando el numerador en $x = -2$

$$
    \text{Resto} = 4 \cdot (-2)^{40} + 8 \cdot (-2)^{39} + 1
\\\
$$
$$
    \text{Resto} = 2^{2} \cdot (2)^{40} - 2^{3} \cdot (2)^{39} + 1
\\\
$$
$$
    \text{Resto} = (2)^{42} - (2)^{42} + 1
\\\
$$
$$
    \text{Resto} = \cancel{(2)^{42}} - \cancel{(2)^{42}} + 1
\\\
$$
$$
    \text{Resto} = 1
$$


