
## Demostracion Coseno de una suma de angulos

$$
    {\color{#777} h} = \cos({\color{#0000ff} \alpha} + {\color{#9005a5} \beta}) + {\color{#777} g}
$$

$$
    \cos({\color{#0000ff} \alpha} + {\color{#9005a5} \beta}) = {\color{#777} h} - {\color{#777} g}
$$

#### Segmento ${\color{#777} h}$ : 
 
$$
    \cos({\color{#0000ff} \alpha}) = \frac{{\color{#777} h}}{\cos({\color{#9005a5} \beta})}
$$  
$$
    {\color{#777} h} = \cos({\color{#0000ff} \alpha}) \cdot \cos({\color{#9005a5} \beta}) 
$$ 




#### Segmento ${\color{#777} g}$ :

$$
    \sin({\color{#0000ff} \alpha}) = \frac{{\color{#777} g}}{\sin({\color{#9005a5} \beta})}
$$
 
$$
    {\color{#777} g} = \sin({\color{#9005a5} \beta}) \cdot \sin({\color{#0000ff} \alpha}) 
$$


#### Por lo tanto:

$$
    \cos({\color{#0000ff} \alpha} + {\color{#9005a5} \beta}) = \cos({\color{#0000ff} \alpha}) \cdot \cos({\color{#9005a5} \beta}) - \sin({\color{#9005a5} \beta}) \cdot \sin({\color{#0000ff} \alpha})
$$

